WIP: fixing invariant

theories/sim/cmra.v
@@ -5,42 +5,40 @@ From stbor.lang Require Export lang.
 
 Set Default Proof Using "Type".
 
+(** Tag map that connect tags to the heaplet that they govern *)
 Inductive tag_kind := tkUnique | tkPub.
 (* Ex() + Ag() *)
 Definition tagKindR := csumR (exclR unitO) unitR.
 
-Definition to_tagKindR (tk: tag_kind) : tagKindR :=
+Definition to_tgkR (tk: tag_kind) : tagKindR :=
   match tk with tkUnique => Cinl (Excl ()) | tkPub => Cinr () end.
 
-Inductive call_state := csOwned (T: gset ptr_id) | csPub.
-(* Ex(ptr_id) + Ag() *)
-Definition callStateR := csumR (exclR (gsetO ptr_id)) unitR.
-
-Definition to_callStateR (cs: call_state) : callStateR :=
-  match cs with csOwned T => Cinl (Excl T) | csPub => Cinr () end.
-
-Definition cmap := gmap call_id call_state.
-(* call_id ⇀ CallState *)
-Definition cmapUR := gmapUR call_id callStateR.
-
-Definition to_cmapUR (cm: cmap) : cmapUR := fmap to_callStateR cm.
-
-Notation heaplet := mem.
+Definition heaplet := gmap loc (scalar * scalar).
 Definition tmap := gmap ptr_id (tag_kind * heaplet).
-Definition heapletR := gmapR loc (agreeR scalarC).
-(* ptr_id ⇀ TagKid x (loc ⇀ Ag(Scalar)) *)
+Definition heapletR := gmapR loc (agreeR (prodO scalarO scalarO)).
+(* ptr_id ⇀ TagKind * (loc ⇀ Ag(Scalar * Scalar)) *)
 Definition tmapUR := gmapUR ptr_id (prodR tagKindR heapletR).
 
-Definition to_heapR (h: heaplet) : heapletR := fmap to_agree h.
-Definition to_tmapUR (pm: tmap) : tmapUR :=
-  fmap (λ tm, (to_tagKindR tm.1, to_heapR tm.2)) pm.
+Definition to_hplR (h: heaplet) : heapletR := fmap to_agree h.
+Definition to_tmUR (tm: tmap) : tmapUR :=
+  fmap (λ kh, (to_tgkR kh.1, to_hplR kh.2)) tm.
 
-Definition lmap := gmap loc ptr_id.
-Definition tagR := exclR (leibnizO ptr_id).
-Definition lmapUR := gmapUR loc tagR.
-Definition to_tagR (t: ptr_id) := Excl t.
 
-Definition res := (tmap * cmap * lmap)%type.
+Definition tag_locs := gmap ptr_id (gset loc).
+
+(** CallId map that protects tags and their associated heaplet *)
+(* Ex(tag ⇀ gset loc) *)
+Definition callStateR := exclR (gmapO ptr_id (gsetO loc)).
+Definition cmap := gmap call_id tag_locs.
+(* call_id ⇀ CallState *)
+Definition cmapUR := gmapUR call_id callStateR.
+Definition to_cmUR (cm: cmap) : cmapUR := fmap Excl cm.
+
+(** Local map that protects tags and their associated heaplet *)
+Definition lmapUR := gmapUR ptr_id (exclR (gsetO loc)).
+Definition to_lmUR (lm: tag_locs) : lmapUR := fmap Excl lm.
+
+Definition res := (tmap * cmap * tag_locs)%type.
 Definition resUR := prodUR (prodUR tmapUR cmapUR) lmapUR.
 
 Definition rtm (r: resUR) : tmapUR := r.1.1.
@@ -62,6 +60,9 @@ Proof.
 Qed.
 
 (** tag_kind properties *)
+Lemma to_tgkR_valid k : valid (to_tgkR k).
+Proof. by destruct k. Qed.
+
 Lemma tag_kind_incl_eq (k1 k2: tagKindR):
   ✓ k2 → k1 ≼ k2 → k1 ≡ k2.
 Proof.
@@ -71,7 +72,7 @@ Proof.
 Qed.
 
 Lemma tagKindR_exclusive (h0 h: heapletR) mb :
-  mb ⋅ Some (to_tagKindR tkUnique, h0) ≡ Some (to_tagKindR tkPub, h) → False.
+  mb ⋅ Some (to_tgkR tkUnique, h0) ≡ Some (to_tgkR tkPub, h) → False.
 Proof.
   destruct mb as [[k ?]|]; [rewrite -Some_op pair_op|rewrite left_id];
     intros [Eq _]%Some_equiv_inj.
@@ -80,7 +81,7 @@ Proof.
 Qed.
 
 Lemma tagKindR_exclusive_2 (h0 h: heapletR) mb :
-  mb ⋅ Some (to_tagKindR tkPub, h0) ≡ Some (to_tagKindR tkUnique, h) → False.
+  mb ⋅ Some (to_tgkR tkPub, h0) ≡ Some (to_tgkR tkUnique, h) → False.
 Proof.
   destruct mb as [[k ?]|]; [rewrite -Some_op pair_op|rewrite left_id];
     intros [Eq _]%Some_equiv_inj.
@@ -89,7 +90,7 @@ Proof.
 Qed.
 
 Lemma tagKindR_exclusive_heaplet' (h0 h: heapletR) mb k1 :
-  mb ⋅ Some (to_tagKindR tkUnique, h0) ≡ Some (to_tagKindR k1, h) →
+  mb ⋅ Some (to_tgkR tkUnique, h0) ≡ Some (to_tgkR k1, h) →
   h0 ≡ h ∧ k1 = tkUnique.
 Proof.
   destruct mb as [[k ?]|]; [rewrite -Some_op pair_op|rewrite left_id];
@@ -99,14 +100,14 @@ Proof.
 Qed.
 
 Lemma tagKindR_exclusive_heaplet (h0 h: heapletR) mb :
-  Some mb ⋅ Some (to_tagKindR tkUnique, h0) ≡ Some (to_tagKindR tkUnique, h) → False.
+  Some mb ⋅ Some (to_tgkR tkUnique, h0) ≡ Some (to_tgkR tkUnique, h) → False.
 Proof.
   destruct mb as [c ]. rewrite -Some_op pair_op. intros [Eq _]%Some_equiv_inj.
   destruct c; inversion Eq; simpl in *; simplify_eq.
 Qed.
 
 Lemma tagKindR_valid (k: tagKindR) :
-  valid k → ∃ k', k = to_tagKindR k'.
+  valid k → ∃ k', k = to_tgkR k'.
 Proof.
   destruct k as [[[]|]|[]|]; [|done|..|done]; intros VAL.
   - by exists tkUnique.
@@ -114,94 +115,76 @@ Proof.
 Qed.
 
 (** cmap properties *)
-Lemma cmap_lookup_op_r (cm1 cm2: cmapUR) c T (VALID: ✓ (cm1 ⋅ cm2)):
-  cm2 !! c = Some (to_callStateR (csOwned T)) →
-  (cm1 ⋅ cm2) !! c = Some (to_callStateR (csOwned T)).
+Lemma cmap_lookup_op_r (cm1 cm2: cmapUR) c (Tls: tag_locs)
+  (VALID: ✓ (cm1 ⋅ cm2)) :
+  cm2 !! c = Some (Excl Tls) → (cm1 ⋅ cm2) !! c = Some (Excl Tls).
 Proof.
   intros HL. move : (VALID c). rewrite lookup_op HL.
   destruct (cm1 !! c) as [cs'|] eqn:Eqc; rewrite Eqc; [|done].
   rewrite -Some_op Some_valid.
-  destruct cs' as [[]|c2|]; auto; try inversion 1.
+  destruct cs'; auto; try inversion 1.
 Qed.
 
-Lemma cmap_lookup_op_l (cm1 cm2: cmapUR) c T (VALID: ✓ (cm1 ⋅ cm2)):
-  cm1 !! c = Some (to_callStateR (csOwned T)) →
-  (cm1 ⋅ cm2) !! c = Some (to_callStateR (csOwned T)).
+Lemma cmap_lookup_op_l (cm1 cm2: cmapUR) c (Tls: tag_locs)
+  (VALID: ✓ (cm1 ⋅ cm2)) :
+  cm1 !! c = Some (Excl Tls) → (cm1 ⋅ cm2) !! c = Some (Excl Tls).
 Proof.
   intros HL. move : (VALID c). rewrite lookup_op HL.
   destruct (cm2 !! c) as [cs'|] eqn:Eqc; rewrite Eqc; [|done].
   rewrite -Some_op Some_valid.
-  destruct cs' as [[]|c2|]; auto; try inversion 1.
+  destruct cs'; auto; try inversion 1.
 Qed.
 
-Lemma cmap_lookup_op_l_equiv (cm1 cm2: cmapUR) c T (VALID: ✓ (cm1 ⋅ cm2)):
-  cm1 !! c ≡ Some (to_callStateR (csOwned T)) →
-  (cm1 ⋅ cm2) !! c ≡ Some (to_callStateR (csOwned T)).
+Lemma cmap_lookup_op_l_equiv (cm1 cm2: cmapUR) c (Tls: tag_locs)
+  (VALID: ✓ (cm1 ⋅ cm2)) :
+  cm1 !! c ≡ Some (Excl Tls) → (cm1 ⋅ cm2) !! c ≡ Some (Excl Tls).
 Proof.
   intros HL. move : (VALID c). rewrite lookup_op HL.
   destruct (cm2 !! c) as [cs'|] eqn:Eqc; rewrite Eqc; [|done].
   rewrite -Some_op Some_valid.
-  destruct cs' as [[]|c2|]; auto; try inversion 1.
+  destruct cs'; auto; try inversion 1.
 Qed.
 
-Lemma cmap_lookup_op_unique_included (cm1 cm2: cmapUR)
-  c T (VALID: ✓ cm2) (INCL: cm1 ≼ cm2):
-  cm1 !! c ≡ Some (to_callStateR (csOwned T)) →
-  cm2 !! c ≡ Some (to_callStateR (csOwned T)).
+Lemma cmap_lookup_op_unique_included (cm1 cm2: cmapUR) c (Tls: tag_locs)
+  (VALID: ✓ cm2) (INCL: cm1 ≼ cm2) :
+  cm1 !! c ≡ Some (Excl Tls) → cm2 !! c ≡ Some (Excl Tls).
 Proof.
   destruct INCL as [cm' Eq]. rewrite Eq. apply cmap_lookup_op_l_equiv.
   by rewrite -Eq.
 Qed.
 
-Lemma cmap_lookup_op_l_equiv_pub (cm1 cm2: cmapUR) c (VALID: ✓ (cm1 ⋅ cm2)):
-  cm1 !! c ≡ Some (to_callStateR csPub) →
-  (cm1 ⋅ cm2) !! c ≡ Some (to_callStateR csPub).
-Proof.
-  intros HL. move : (VALID c). rewrite lookup_op HL.
-  destruct (cm2 !! c) as [cs'|] eqn:Eqc; rewrite Eqc; [|done].
-  rewrite -Some_op Some_valid.
-  destruct cs' as [[]|c2|]; auto; inversion 1.
-Qed.
-
-Lemma cmap_insert_op_r (cm1 cm2: cmapUR) c T cs (VALID: ✓ (cm1 ⋅ cm2)):
-  cm2 !! c = Some (to_callStateR (csOwned T)) →
+Lemma cmap_insert_op_r (cm1 cm2: cmapUR) c Tls cs
+  (VALID: ✓ (cm1 ⋅ cm2)):
+  cm2 !! c = Some (Excl Tls) →
   cm1 ⋅ <[c:=cs]> cm2 = <[c:=cs]> (cm1 ⋅ cm2).
 Proof.
   intros HL. apply (map_eq (cm1 ⋅ <[c:=cs]> cm2)). intros c'.
   move : (VALID c). rewrite 2!lookup_op HL.
-  destruct (cm1 !! c) as [[| |]|] eqn:Eqc; rewrite Eqc; [inversion 1..|].
+  destruct (cm1 !! c) eqn:Eqc; rewrite Eqc; [inversion 1..|].
   intros VL.
   case (decide (c' = c)) => [->|?].
   - by rewrite 2!lookup_insert Eqc.
   - do 2 (rewrite lookup_insert_ne //). by rewrite lookup_op.
 Qed.
 
-Lemma callStateR_exclusive_2 T mb :
-  mb ⋅ Some (to_callStateR csPub) ≡ Some (to_callStateR (csOwned T)) → False.
-Proof.
-  destruct mb as [cs|]; [rewrite -Some_op|rewrite left_id];
-    intros Eq%Some_equiv_inj.
-  - destruct cs; inversion Eq.
-  - inversion Eq.
-Qed.
-
-Lemma callStateR_exclusive_Some T1 T2 cs :
-  Some cs ⋅ Some (to_callStateR (csOwned T1)) ≡ Some (to_callStateR (csOwned T2)) → False.
+Lemma callStateR_exclusive_Some (Tls1 Tls2: tag_locs) (cs: callStateR) :
+  Some cs ⋅ Some (Excl Tls1) ≡ Some (Excl Tls2) → False.
 Proof.
   rewrite -Some_op. intros Eq%Some_equiv_inj.
-  destruct cs as [[]| |]; inversion Eq; simplify_eq.
+  destruct cs; inversion Eq; simplify_eq.
 Qed.
 
-Lemma callStateR_exclusive_eq T1 T2 mb :
-  mb ⋅ Some (to_callStateR (csOwned T1)) ≡ Some (to_callStateR (csOwned T2)) → T1 = T2.
+Lemma callStateR_exclusive_eq (Tls1 Tls2: tag_locs) mb :
+  mb ⋅ Some (Excl Tls1) ≡ Some (Excl Tls2) → Tls1 = Tls2.
 Proof.
   destruct mb. by intros ?%callStateR_exclusive_Some.
   rewrite left_id. intros Eq%Some_equiv_inj. by simplify_eq.
 Qed.
 
 (** tmap properties *)
-Lemma tmap_insert_op_r (pm1 pm2: tmapUR) t h0 kh (VALID: ✓ (pm1 ⋅ pm2)):
-  pm2 !! t = Some (to_tagKindR tkUnique, h0) →
+Lemma tmap_insert_op_r (pm1 pm2: tmapUR) t h0 kh
+  (VALID: ✓ (pm1 ⋅ pm2)) :
+  pm2 !! t = Some (to_tgkR tkUnique, h0) →
   pm1 ⋅ <[t:=kh]> pm2 = <[t:=kh]> (pm1 ⋅ pm2).
 Proof.
   intros HL. apply (map_eq (pm1 ⋅ <[t:=kh]> pm2)). intros t'.
@@ -214,81 +197,84 @@ Proof.
     + do 2 (rewrite lookup_insert_ne //). by rewrite lookup_op.
 Qed.
 
-Lemma tmap_lookup_op_r (pm1 pm2: tmapUR) t h0 (VALID: ✓ (pm1 ⋅ pm2)):
-  pm2 !! t = Some (to_tagKindR tkUnique, h0) →
-  (pm1 ⋅ pm2) !! t = Some (to_tagKindR tkUnique, h0).
+Lemma tmap_lookup_op_r (pm1 pm2: tmapUR) t h0
+  (VALID: ✓ (pm1 ⋅ pm2)) :
+  pm2 !! t = Some (to_tgkR tkUnique, h0) →
+  (pm1 ⋅ pm2) !! t = Some (to_tgkR tkUnique, h0).
 Proof.
   intros HL. move : (VALID t). rewrite lookup_op HL.
   destruct (pm1 !! t) as [[k1 h1]|] eqn:Eqt; rewrite Eqt; [|done].
   rewrite -Some_op pair_op. intros [?%exclusive_r]; [done|apply _].
 Qed.
 
-Lemma tmap_lookup_op_r_unique_equiv (pm1 pm2: tmapUR) t h0 (VALID: ✓ (pm1 ⋅ pm2)):
-  pm2 !! t ≡ Some (to_tagKindR tkUnique, h0) →
-  (pm1 ⋅ pm2) !! t ≡ Some (to_tagKindR tkUnique, h0).
-Proof.
-  intros HL. move : (VALID t). rewrite lookup_op HL.
-  destruct (pm1 !! t) as [[k1 h1]|] eqn:Eqt; rewrite Eqt; [|done].
-  rewrite -Some_op pair_op. intros [?%exclusive_r]; [done|apply _].
-Qed.
-
-Lemma tmap_lookup_op_l_unique_equiv (pm1 pm2: tmapUR) t h0
+Lemma tmap_lookup_op_l_uniq_equiv (pm1 pm2: tmapUR) t h0
   (VALID: ✓ (pm1 ⋅ pm2)):
-  pm1 !! t ≡ Some (to_tagKindR tkUnique, h0) →
-  (pm1 ⋅ pm2) !! t ≡ Some (to_tagKindR tkUnique, h0).
+  pm1 !! t ≡ Some (to_tgkR tkUnique, h0) →
+  (pm1 ⋅ pm2) !! t ≡ Some (to_tgkR tkUnique, h0).
 Proof.
   intros HL. move : (VALID t). rewrite lookup_op HL.
   destruct (pm2 !! t) as [[k2 h2]|] eqn:Eqt; rewrite Eqt; [|done].
   rewrite -Some_op pair_op. intros [?%exclusive_l]; [done|apply _].
 Qed.
 
-Lemma tmap_lookup_op_unique_included (pm1 pm2: tmapUR) t h0
+Lemma tmap_lookup_op_uniq_included (pm1 pm2: tmapUR) t h0
   (VALID: ✓ pm2) (INCL: pm1 ≼ pm2):
-  pm1 !! t ≡ Some (to_tagKindR tkUnique, h0) →
-  pm2 !! t ≡ Some (to_tagKindR tkUnique, h0).
+  pm1 !! t ≡ Some (to_tgkR tkUnique, h0) →
+  pm2 !! t ≡ Some (to_tgkR tkUnique, h0).
 Proof.
-  destruct INCL as [cm' Eq]. rewrite Eq. apply tmap_lookup_op_l_unique_equiv.
+  destruct INCL as [cm' Eq]. rewrite Eq. apply tmap_lookup_op_l_uniq_equiv.
   by rewrite -Eq.
 Qed.
 
-Lemma tmap_lookup_op_r_equiv_pub (pm1 pm2: tmapUR) t h2 (VALID: ✓ (pm1 ⋅ pm2)):
-  pm2 !! t ≡ Some (to_tagKindR tkPub, h2) →
-  ∃ h1, (pm1 ⋅ pm2) !! t ≡ Some (to_tagKindR tkPub, h1 ⋅ h2).
+Lemma tmap_lookup_op_r_uniq_equiv (pm1 pm2: tmapUR) t h0
+  (VALID: ✓ (pm1 ⋅ pm2)) :
+  pm2 !! t ≡ Some (to_tgkR tkUnique, h0) →
+  (pm1 ⋅ pm2) !! t ≡ Some (to_tgkR tkUnique, h0).
+Proof.
+  intros HL. eapply tmap_lookup_op_uniq_included; [done|..|exact HL].
+  by apply cmra_included_r.
+Qed.
+
+
+Lemma tmap_lookup_op_r_equiv_pub (pm1 pm2: tmapUR) t h2
+  (VALID: ✓ (pm1 ⋅ pm2)):
+  pm2 !! t ≡ Some (to_tgkR tkPub, h2) →
+  ∃ h1, (pm1 ⋅ pm2) !! t ≡ Some (to_tgkR tkPub, h1 ⋅ h2).
 Proof.
   intros HL. move : (VALID t). rewrite lookup_op.
   destruct (pm1 !! t) as [[k1 h1]|] eqn:Eqt; rewrite Eqt; rewrite -> HL.
   - rewrite -Some_op pair_op. move => [ VL1 ?]. exists h1. simpl in VL1.
     rewrite HL -Some_op pair_op.
-    by rewrite -(tag_kind_incl_eq (to_tagKindR tkPub) _ VL1 (cmra_included_r _ _)).
+    by rewrite -(tag_kind_incl_eq (to_tgkR tkPub) _ VL1 (cmra_included_r _ _)).
   - intros _. exists (∅: gmap loc _). by rewrite 2!left_id HL.
 Qed.
 
 Lemma tmap_valid (r_f r: tmapUR) t h0 kh
-  (Eqtg: r !! t = Some (to_tagKindR tkUnique, h0)) (VN: ✓ kh) :
+  (Eqtg: r !! t = Some (to_tgkR tkUnique, h0)) (VN: ✓ kh) :
   ✓ (r_f ⋅ r) → ✓ (r_f ⋅ (<[t:= kh]> r)).
 Proof.
   intros VALID.
   apply (local_update_discrete_valid_frame _ _ _ VALID).
   have EQ := (tmap_insert_op_r _ _ _ _ kh VALID Eqtg). rewrite EQ.
   eapply (insert_local_update _ _ _
-          (to_tagKindR tkUnique, h0) (to_tagKindR tkUnique, h0));
+          (to_tgkR tkUnique, h0) (to_tgkR tkUnique, h0));
           [|exact Eqtg|by apply exclusive_local_update].
   by rewrite (tmap_lookup_op_r _ _ _ _ VALID Eqtg).
 Qed.
 
 (** heaplet *)
-Lemma to_heapR_valid h : ✓ (to_heapR h).
+Lemma to_hplR_valid h : ✓ (to_hplR h).
 Proof.
-  intros l. rewrite /to_heapR lookup_fmap.
+  intros l. rewrite /to_hplR lookup_fmap.
   destruct (h !! l) eqn:Eq; rewrite Eq //.
 Qed.
 
-Lemma to_heapR_lookup h l s :
-  to_heapR h !! l ≡ Some (to_agree s) → h !! l = Some s.
+Lemma to_hplR_lookup h l s :
+  to_hplR h !! l ≡ Some (to_agree s) → h !! l = Some s.
 Proof.
-  rewrite /to_heapR lookup_fmap.
+  rewrite /to_hplR lookup_fmap.
   destruct (h !! l) as [s'|] eqn:Eqs; rewrite Eqs /=; [|by inversion 1].
-  intros Eq%Some_equiv_inj%to_agree_inj. by inversion Eq.
+  intros Eq%Some_equiv_inj%to_agree_inj%leibniz_equiv_iff. by subst s'.
 Qed.
 
 Lemma heapletR_elem_of_dom (h: heapletR) l (VALID: valid h) :
@@ -299,7 +285,7 @@ Proof.
 Qed.
 
 (** lmap *)
-Lemma lmap_lookup_op_r (lm1 lm2 : lmapUR) (VALID: ✓ (lm1 ⋅ lm2)) l ls :
+(* Lemma lmap_lookup_op_r (lm1 lm2 : lmapUR) (VALID: ✓ (lm1 ⋅ lm2)) l ls :
   lm2 !! l ≡ Some ls → ((lm1 ⋅ lm2) !! l : optionR tagR) ≡ Some ls.
 Proof.
   intros Eq. move : (VALID l). rewrite lookup_op Eq.
@@ -341,7 +327,7 @@ Proof.
   have VALID: valid (Some c ⋅ mb) by rewrite Eq. move :Eq.
   destruct c, mb as [[]|]; simplify_eq; try done.
   rewrite right_id. by intros ?%Some_equiv_inj.
-Qed.
+Qed. *)
 
 (** The Core *)
 
@@ -353,77 +339,78 @@ Proof.
 Qed.
 
 Lemma tmap_lookup_core_pub (pm: tmapUR) t h:
-  pm !! t ≡ Some (to_tagKindR tkPub, h) →
-  core pm !! t ≡ Some (to_tagKindR tkPub, h).
+  pm !! t ≡ Some (to_tgkR tkPub, h) →
+  core pm !! t ≡ Some (to_tgkR tkPub, h).
 Proof. intros Eq. rewrite lookup_core Eq /core /= core_id //. Qed.
 
 (** Resources that we own. *)
 
 Definition res_tag tg tk (h: heaplet) : resUR :=
-  ({[tg := (to_tagKindR tk, to_agree <$> h)]}, ε, ε).
+  ({[tg := (to_tgkR tk, to_agree <$> h)]}, ε, ε).
 
-Definition res_callState (c: call_id) (cs: call_state) : resUR :=
-  (ε, {[c := to_callStateR cs]}, ε).
+Definition res_cs (c: call_id) (cs: tag_locs) : resUR :=
+  (ε, to_cmUR {[c := cs]}, ε).
 
-
-Fixpoint write_local (l:loc) (n:nat) (t: ptr_id) (ls: lmap) : lmap :=
+Fixpoint locs_seq (l:loc) (n:nat) : gset loc :=
   match n with
-  | O => ls
-  | S n => <[l := t]>(write_local (l +ₗ 1) n t ls)
+  | O => ∅
+  | S n => {[l]} ∪ locs_seq (l +ₗ 1) n
   end.
 
-Definition res_loc l n t : resUR := (ε, to_tagR <$> (write_local l n t ∅)).
+Definition res_loc l n t : resUR := (ε, to_lmUR {[t := locs_seq l n]}).
 
-Definition res_mapsto (l:loc) (v: value) (t: ptr_id) : resUR :=
-  res_loc l (length v) t ⋅ res_tag t tkUnique (write_mem l v ∅).
+Fixpoint write_hpl l (v: list (scalar * scalar)) (h: heaplet) : heaplet :=
+  match v with
+  | [] => h
+  | sst :: v' => write_hpl (l +ₗ 1) v' (<[l:=sst]> h)
+  end.
+
+Definition res_mapsto (l:loc) (v: list (scalar * scalar)) (t: ptr_id) : resUR :=
+  res_loc l (length v) t ⋅ res_tag t tkUnique (write_hpl l v ∅).
 
 (** res_tag *)
-Lemma res_tag_alloc_local_update lsf t k h (FRESH: lsf.(rtm) !! t = None) :
+Lemma res_tag_alloc_local_update lsf t k h
+  (FRESH: lsf.(rtm) !! t = None) :
   (lsf, ε) ~l~> (lsf ⋅ res_tag t k h, res_tag t k h).
 Proof.
   destruct lsf as [[tm cm] lm]. rewrite 2!pair_op right_id right_id.
   apply prod_local_update_1, prod_local_update_1.
   rewrite cmra_comm -insert_singleton_op //.
   apply alloc_singleton_local_update; [done|].
-  split. by destruct k. apply to_heapR_valid.
+  split. by destruct k. apply to_hplR_valid.
 Qed.
 
-
-Lemma res_tag_unique_pub_local_update (r: resUR) t h
-  (NONE: r.(rtm) !! t = None) :
-  (r ⋅ res_tag t tkUnique h, res_tag t tkUnique h) ~l~>
-  (r ⋅ res_tag t tkPub ∅, res_tag t tkPub ∅).
+Lemma res_tag_uniq_insert_local_update_inner (tm: tmapUR) t k2 (h1 h2: heaplet):
+  tm !! t = None →
+  (tm ⋅ {[t := (to_tgkR tkUnique, to_hplR h1)]},
+    {[t := (to_tgkR tkUnique, to_hplR h1)]}) ~l~>
+  (tm ⋅ {[t := (to_tgkR k2, to_hplR h2)]}, {[t := (to_tgkR k2, to_hplR h2)]}).
 Proof.
-  destruct r as [[tm cm] lm].
-  apply prod_local_update_1, prod_local_update_1. rewrite /=.
-  do 2 rewrite (cmra_comm tm) -insert_singleton_op //.
-  rewrite -(insert_insert tm t (Cinr (), to_agree <$> ∅)
-                               (Cinl (Excl ()), to_agree <$> h)).
-  eapply (singleton_local_update (<[t := _]> tm : tmapUR)).
-  by rewrite lookup_insert.
-  apply exclusive_local_update. split; [done|apply to_heapR_valid].
-Qed.
-
-Lemma res_tag_insert_local_update (r: resUR) h1 h2 (t: ptr_id)
-  (NONE: r.(rtm) !! t = None):
-  (r ⋅ res_tag t tkUnique h1, res_tag t tkUnique h1) ~l~>
-  (r ⋅ res_tag t tkUnique h2, res_tag t tkUnique h2).
-Proof.
-  destruct r as [[tm cm] lm].
-  apply prod_local_update_1, prod_local_update_1. rewrite /=.
+  intros.
   do 2 rewrite (cmra_comm tm) -insert_singleton_op //.
   rewrite -(insert_insert tm t (_, to_agree <$> h2)
                                (Cinl (Excl ()), to_agree <$> h1)).
   eapply (singleton_local_update (<[t := _]> tm : tmapUR)).
-  by rewrite lookup_insert.
-  apply exclusive_local_update. split; [done|apply to_heapR_valid].
+  - by rewrite lookup_insert.
+  - apply exclusive_local_update.
+    split; [apply to_tgkR_valid|apply to_hplR_valid].
+Qed.
+
+Lemma res_tag_uniq_local_update (r: resUR) t h k' h'
+  (NONE: r.(rtm) !! t = None) :
+  (r ⋅ res_tag t tkUnique h, res_tag t tkUnique h) ~l~>
+  (r ⋅ res_tag t k' h', res_tag t k' h').
+Proof.
+  destruct r as [[tm cm] lm].
+  apply prod_local_update_1, prod_local_update_1. rewrite /=.
+  by apply res_tag_uniq_insert_local_update_inner.
 Qed.
 
 Lemma res_tag_1_insert_local_update (r: resUR) (l: loc) s1 s2 (t: ptr_id)
   (NONE: r.(rtm) !! t = None):
   (r ⋅ res_tag t tkUnique {[l := s1]}, res_tag t tkUnique {[l := s1]}) ~l~>
   (r ⋅ res_tag t tkUnique {[l := s2]}, res_tag t tkUnique {[l := s2]}).
-Proof. by apply res_tag_insert_local_update. Qed.
+Proof. by apply res_tag_uniq_local_update. Qed.
 
 Lemma res_tag_1_insert_local_update_r (r: resUR) r' (l: loc) s1 s2 (t: ptr_id)
   (NONE: r.(rtm) !! t = None):
@@ -432,16 +419,11 @@ Lemma res_tag_1_insert_local_update_r (r: resUR) r' (l: loc) s1 s2 (t: ptr_id)
 Proof.
   destruct r as [[tm cm] lm].
   apply prod_local_update_1, prod_local_update_1. rewrite /= 2!left_id.
-  do 2 rewrite (cmra_comm tm) -insert_singleton_op //.
-  rewrite -(insert_insert tm t (_, to_agree <$> {[l := s2]})
-                               (Cinl (Excl ()), to_agree <$> {[l := s1]})).
-  eapply (singleton_local_update (<[t := _]> tm : tmapUR)).
-  by rewrite lookup_insert.
-  apply exclusive_local_update. split; [done|apply to_heapR_valid].
+  by apply (res_tag_uniq_insert_local_update_inner _ _ tkUnique).
 Qed.
 
 Lemma res_tag_lookup (k: tag_kind) (h: heaplet) (t: ptr_id) :
-  (res_tag t k h).(rtm) !! t ≡ Some (to_tagKindR k, to_agree <$> h).
+  (res_tag t k h).(rtm) !! t ≡ Some (to_tgkR k, to_agree <$> h).
 Proof. by rewrite lookup_insert. Qed.
 
 Lemma res_tag_lookup_ne (k: tag_kind) (h: heaplet) (t t': ptr_id) (NEQ: t' ≠ t) :
@@ -449,223 +431,89 @@ Lemma res_tag_lookup_ne (k: tag_kind) (h: heaplet) (t t': ptr_id) (NEQ: t' ≠ t
 Proof. by rewrite lookup_insert_ne. Qed.
 
 (** res_mapsto *)
-Lemma write_local_lookup l n t ls :
-  (∀ (i: nat), (i < n)%nat →
-    write_local l n t ls !! (l +ₗ i) = Some t) ∧
-  (∀ (l': loc), (∀ (i: nat), (i < n)%nat → l' ≠ l +ₗ i) →
-    write_local l n t ls !! l' = ls !! l').
-Proof.
-  revert l ls. induction n as [|n IH]; intros l ls; simpl.
-  { split; intros ??; [lia|done]. }
-  destruct (IH (l +ₗ 1) ls) as [IH1 IH2].
-  split.
-  - intros i Lt. destruct i as [|i].
-    + rewrite shift_loc_0_nat lookup_insert //.
-    + have Eql: l +ₗ S i = (l +ₗ 1) +ₗ i.
-      { rewrite shift_loc_assoc. f_equal. lia. }
-      rewrite lookup_insert_ne.
-      * rewrite Eql. destruct (IH (l +ₗ 1) ls) as [IH' _].
-        apply IH'; lia.
-      * rewrite -{1}(shift_loc_0_nat l). intros ?%shift_loc_inj. lia.
-  - intros l' Lt. rewrite lookup_insert_ne.
-    + apply IH2. intros i Lt'.
-      rewrite (_: (l +ₗ 1) +ₗ i = l +ₗ S i); last first.
-      { rewrite shift_loc_assoc. f_equal. lia. }
-      apply Lt. lia.
-    + specialize (Lt O ltac:(lia)). by rewrite shift_loc_0_nat in Lt.
-Qed.
 
-Lemma write_local_lookup_case l n t ls :
-  ∀ l' t', write_local l n t ls !! l' = Some t' →
-  ls !! l' = Some t' ∧ (∀ i : nat, (i < n)%nat → l' ≠ l +ₗ i) ∨
-  ∃ i, (0 ≤ i < n) ∧ l' = l +ₗ i.
-Proof.
-  destruct (write_local_lookup l n t ls) as [EQ1 EQ2].
-  intros l1 t1s1 Eq'.
-  case (decide (l1.1 = l.1)) => [Eql|NEql];
-    [case (decide (l.2 ≤ l1.2 < l.2 + n)) => [[Le Lt]|NIN]|].
-  - have Eql2: l1 = l +ₗ Z.of_nat (Z.to_nat (l1.2 - l.2)). {
-      destruct l, l1. move : Eql Le => /= -> ?.
-      rewrite /shift_loc /= Z2Nat.id; [|lia]. f_equal. lia. }
-    right. rewrite Eql2. eexists; split; [|done].
-    rewrite Eql2 /= in Lt. lia.
-  - left.
-    have ?: ∀ i : nat, (i < n)%nat → l1 ≠ l +ₗ i.
-    { intros i Lt Eq3. apply NIN. rewrite Eq3 /=. lia. }
-     rewrite EQ2 // in Eq'.
-  - left.
-    have ?: ∀ i : nat, (i < n)%nat → l1 ≠ l +ₗ i.
-    { intros i Lt Eq3. apply NEql. by rewrite Eq3. }
-    rewrite EQ2 // in Eq'.
-Qed.
+Lemma res_loc_lookup l n t :
+  (res_loc l n t).(rlm) !! t ≡ Some (Excl $ locs_seq l n).
+Proof. rewrite /= lookup_fmap lookup_insert //. Qed.
 
 Lemma res_mapsto_llookup l v t :
-  (∀ (i: nat), (i < length v)%nat →
-    (res_mapsto l v t).(rlm) !! (l +ₗ i) = Some $ to_tagR t) ∧
-  (∀ (l': loc), (∀ (i: nat), (i < length v)%nat → l' ≠ l +ₗ i) →
-    (res_mapsto l v t).(rlm) !! l' = None).
-Proof.
-  destruct (write_local_lookup l (length v) t ∅) as [EQ1 EQ2]. split.
-  - intros i Lti. by rewrite /= right_id lookup_fmap (EQ1 _ Lti).
-  - intros l' NEQ. by rewrite /= right_id lookup_fmap (EQ2 _ NEQ).
-Qed.
-
-Lemma res_mapsto_llookup_case l v t :
-  ∀ l' t', ((res_mapsto l v t).(rlm) !! l' : optionR tagR) ≡ Some t' →
-  t' = to_tagR t ∧ ∃ i, (0 ≤ i < length v) ∧ l' = l +ₗ i.
-Proof.
-  intros l' t' Eq'. apply leibniz_equiv_iff in Eq'.
-  move : Eq'. rewrite /= right_id lookup_fmap.
-  destruct (write_local l (length v) t ∅ !! l')
-    as [t1|] eqn:Eql'; rewrite Eql'; [|done].
-  simpl. intros. simplify_eq.
-  destruct (write_local_lookup_case _ _ _ _ _ _ Eql') as [[]|Eq']; [done|].
-  destruct Eq' as [i [[? Lti] Eqi]].
-  have Lti': (Z.to_nat i < length v)%nat by rewrite Nat2Z.inj_lt Z2Nat.id.
-  destruct (write_local_lookup l (length v) t ∅) as [EQ _].
-  specialize (EQ _ Lti'). rewrite Z2Nat.id // -Eqi Eql' in EQ. simplify_eq.
-  naive_solver.
-Qed.
-
-Lemma res_loc_lookup_1 l n t (LEN: (0 < n)%nat) :
-  ((res_loc l n t).(rlm) !! l : optionR tagR) ≡ Some (to_tagR t).
-Proof. rewrite /= lookup_fmap. destruct n; [lia|]. rewrite /= lookup_insert //. Qed.
-
-Lemma res_mapsto_llookup_1 l v t (LEN: (0 < length v)%nat) :
-  ((res_mapsto l v t).(rlm) !! l : optionR tagR) ≡ Some (to_tagR t).
-Proof. rewrite lookup_op res_loc_lookup_1 //. Qed.
+  (res_mapsto l v t).(rlm) !! t ≡ Some (Excl $ locs_seq l (length v)).
+Proof. rewrite lookup_op res_loc_lookup //. Qed.
 
 Lemma res_mapsto_tlookup l v (t: ptr_id) :
   (res_mapsto l v t).(rtm) !! t ≡
-    Some (to_tagKindR tkUnique, to_agree <$> (write_mem l v ∅)).
+    Some (to_tgkR tkUnique, to_agree <$> (write_hpl l v ∅)).
 Proof. by rewrite lookup_op /= lookup_empty left_id lookup_insert. Qed.
 
 Lemma res_mapsto_tlookup_ne l v (t t': ptr_id) (NEQ: t' ≠ t) :
   (res_mapsto l v t).(rtm) !! t' ≡ None.
 Proof. by rewrite lookup_op /= lookup_empty left_id lookup_insert_ne. Qed.
 
-Lemma write_local_plus1 l n t :
-  write_local (l +ₗ 1) n t ∅ !! l = None.
-Proof.
-  destruct (write_local_lookup (l +ₗ 1) n t ∅) as [_ EQ].
-  rewrite EQ //. intros ??. rewrite shift_loc_assoc -{1}(shift_loc_0 l).
-  intros ?%shift_loc_inj. lia.
-Qed.
-
-Lemma write_local_res_S l n t :
-  (to_tagR <$> write_local l (S n) t ∅ : lmapUR) ≡
-  ({[l := to_tagR t]} ⋅ (to_tagR <$> write_local (l +ₗ 1) n t ∅) : lmapUR).
-Proof.
-  rewrite /= fmap_insert /= insert_singleton_op //.
-  rewrite lookup_fmap write_local_plus1 //.
-Qed.
-
-Lemma write_local_mem_dom l n t :
-  dom (gset loc) (write_local l n t ∅) ≡ dom (gset loc) (init_mem l n ∅).
-Proof.
-  revert l. induction n as [|n IH]; simpl; intros l; [done|].
-  rewrite /= 2!dom_insert IH //.
-Qed.
-
 (** allocating locals *)
-Lemma write_local_res_alloc_local_update lsf l n t:
-  (∀ i, (i < n)%nat → lsf !! (l +ₗ i) = None) →
-  (lsf, ε) ~l~>
-  (lsf ⋅ (to_tagR <$> write_local l n t ∅) : lmapUR, to_tagR <$> write_local l n t ∅ : lmapUR).
+
+Lemma res_loc_alloc_local_update (lm: lmapUR) (t: ptr_id) ls :
+  lm !! t = None →
+  (lm, ε) ~l~> (lm ⋅ (to_lmUR {[t := ls]}), (to_lmUR {[t := ls]})).
 Proof.
-  revert l lsf.
-  induction n as [|n IH]; intros l lsf HL.
-  - rewrite /= fmap_empty right_id //.
-  - rewrite /= write_local_res_S.
-    rewrite (cmra_comm ({[l := to_tagR t]} : lmapUR) (to_tagR <$> write_local _ _ _ _)).
-    rewrite cmra_assoc.
-    etrans.
-    + apply (IH (l +ₗ 1)).
-      intros i Lt. rewrite shift_loc_assoc -(Nat2Z.inj_add 1).
-      apply HL. lia.
-    + have NEQ1: write_local (l +ₗ 1) n t ∅ !! l = None.
-      { rewrite {1}/write_local write_local_plus1 //. }
-      have ?: (lsf ⋅ (to_tagR <$> write_local (l +ₗ 1) n t ∅)) !! l = None.
-      { rewrite lookup_op lookup_fmap NEQ1 right_id_L.
-        specialize (HL O). rewrite shift_loc_0_nat in HL. apply HL. lia. }
-      rewrite 2!(cmra_comm _  {[l := _]})
-              -insert_singleton_op // -insert_singleton_op;
-        [|by rewrite lookup_fmap NEQ1].
-      by apply alloc_local_update.
+  intros FRESH.
+  rewrite /to_lmUR fmap_insert fmap_empty insert_empty
+          (cmra_comm _  {[t := _]}) -insert_singleton_op //.
+  by apply alloc_local_update.
 Qed.
 
-Lemma res_mapsto_local_alloc_local_update lsf l v t:
-  lsf.(rtm) !! t = None →
-  (∀ i, (i < length v)%nat → lsf.(rlm) !! (l +ₗ i) = None) →
-  (lsf, ε) ~l~> (lsf ⋅ res_mapsto l v t, res_mapsto l v t).
+Lemma res_mapsto_alloc_local_update r l v t:
+  r.(rtm) !! t = None → r.(rlm) !! t = None →
+  (r, ε) ~l~> (r ⋅ res_mapsto l v t, res_mapsto l v t).
 Proof.
-  intros FRESH1 FRESH2. destruct lsf as [[tm cm] lm].
+  intros FRESH1 FRESH2. destruct r as [[tm cm] lm].
   rewrite /res_mapsto (cmra_comm (res_loc _ _ _)).
-  etrans. by apply (res_tag_alloc_local_update _ t tkUnique (write_mem l v ∅)).
-  rewrite !pair_op !right_id left_id /=. apply prod_local_update_2.
-  by apply write_local_res_alloc_local_update.
+  etrans.
+  - by apply (res_tag_alloc_local_update _ t tkUnique (write_hpl l v ∅)).
+  - rewrite !pair_op !right_id left_id /=.
+    by apply prod_local_update_2, res_loc_alloc_local_update.
 Qed.
 
 (** deallocating locals *)
-Lemma write_local_res_dealloc_local_update (lsf: lmapUR) l n t:
-  (∀ i, (i < n)%nat → lsf !! (l +ₗ i) = None) →
-  (lsf ⋅ (to_tagR <$> write_local l n t ∅) : lmapUR, (to_tagR <$> write_local l n t ∅) : lmapUR) ~l~>
-  (lsf : lmapUR, ε : lmapUR).
+
+Lemma res_loc_dealloc_local_update (lm: lmapUR) t ls:
+  lm !! t = None →
+  (lm ⋅ (to_lmUR {[t := ls]}), to_lmUR {[t := ls]}) ~l~> (lm, ε).
 Proof.
-  revert l lsf.
-  induction n as [|n IH]; intros l lsf HL.
-  - rewrite /= fmap_empty right_id_L //.
-  - rewrite /= write_local_res_S.
-    rewrite (cmra_comm ({[l := to_tagR t]} : lmapUR) (to_tagR <$> write_local _ _ _ _)).
-    rewrite cmra_assoc.
-    have NEQ1: write_local (l +ₗ 1) n t ∅ !! l = None.
-    { rewrite {1}/write_local write_local_plus1 //. }
-    have ?: (lsf ⋅ (to_tagR <$> write_local (l +ₗ 1) n t ∅)) !! l = None.
-    { rewrite lookup_op lookup_fmap NEQ1 right_id_L.
-      specialize (HL O). rewrite shift_loc_0_nat in HL. apply HL. lia. }
-    etrans.
-    + rewrite 2!(cmra_comm _  {[l := _]}) -insert_singleton_op; [|done].
-      rewrite -insert_singleton_op; [|by rewrite lookup_fmap NEQ1].
-      eapply (delete_local_update_cancelable _ _ l); [|by rewrite lookup_insert..].
-      apply _.
-    + rewrite 2!delete_insert_delete delete_notin // delete_notin;
-        [|by rewrite lookup_fmap NEQ1].
-      apply (IH (l +ₗ 1)).
-      intros i Lt. rewrite shift_loc_assoc -(Nat2Z.inj_add 1).
-      apply HL. lia.
+  intros ?.
+  rewrite /to_lmUR fmap_insert fmap_empty insert_empty
+          (cmra_comm _  {[t := _]}) -insert_singleton_op; [|done].
+  etrans.
+  - eapply (delete_local_update_cancelable _ _ t); [|by rewrite lookup_insert..].
+    apply _.
+  - rewrite 2!delete_insert_delete delete_empty delete_notin //.
 Qed.
 
-Lemma res_mapsto_res_tag_public (r: resUR) l v t
-  (NONE1: ∀ i, (i < length v)%nat → r.(rlm) !! (l +ₗ i) = None)
+Lemma res_mapsto_res_tag (r: resUR) l v t k' h'
+  (NONE1: r.(rlm) !! t = None)
   (NONE2: r.(rtm) !! t = None):
   (r ⋅ res_mapsto l v t, res_mapsto l v t) ~l~>
-  (r ⋅ res_tag t tkPub ∅, res_tag t tkPub ∅).
+  (r ⋅ res_tag t k' h', res_tag t k' h').
 Proof.
   rewrite /res_mapsto. destruct r as [[tm cm] lm].
   rewrite (cmra_comm (res_loc _ _ _)) cmra_assoc. etrans.
   - apply prod_local_update_2. rewrite /= right_id left_id.
-    by apply write_local_res_dealloc_local_update.
+    by apply res_loc_dealloc_local_update.
   - rewrite !pair_op /= !right_id.
     apply prod_local_update_1, prod_local_update_1. rewrite /=.
-    do 2 rewrite (cmra_comm tm) -insert_singleton_op //.
-    rewrite -(insert_insert tm t (Cinr (), to_agree <$> ∅)
-                                 (Cinl (Excl ()), to_agree <$> (write_mem l v ∅))).
-    eapply (singleton_local_update (<[t := _]> tm : tmapUR)).
-    by rewrite lookup_insert.
-    apply exclusive_local_update. split; [done|apply to_heapR_valid].
+    by apply (res_tag_uniq_insert_local_update_inner _ _ k').
 Qed.
 
 (** updating locals *)
 Lemma res_mapsto_1_insert_local_update (r: resUR) (l: loc) s1 s2 (t: ptr_id)
-  (NONE1: r.(rlm) !! l = None) (NONE2: r.(rtm) !! t = None):
+  (NONE: r.(rtm) !! t = None) :
   (r ⋅ res_mapsto l [s1] t, res_mapsto l [s1] t) ~l~>
   (r ⋅ res_mapsto l [s2] t, res_mapsto l [s2] t).
 Proof.
   intros. rewrite /res_mapsto cmra_assoc. etrans.
   - eapply res_tag_1_insert_local_update_r.
-    by rewrite lookup_op NONE2 /= lookup_empty right_id_L.
-  - rewrite -(cmra_assoc r) 2!(cmra_comm (res_loc _ _ _)) 2!cmra_assoc.
-    rewrite /= insert_empty //.
+    by rewrite lookup_op NONE /= lookup_empty right_id_L.
+  - rewrite -(cmra_assoc r) 2!(cmra_comm (res_loc _ _ _)) 2!cmra_assoc
+            /= insert_empty //.
 Qed.
 
 Lemma res_mapsto_tdom l v t:
@@ -673,6 +521,17 @@ Lemma res_mapsto_tdom l v t:
 Proof.
   intros t1.
   rewrite elem_of_dom /res_mapsto lookup_op /= left_id elem_of_singleton.
+  case (decide (t1 = t)) => ?.
+  - subst t1. rewrite lookup_insert. naive_solver.
+  - rewrite lookup_insert_ne // lookup_empty. split; [by destruct 1|done].
+Qed.
+
+Lemma res_mapsto_ldom l v t:
+  dom (gset nat) (res_mapsto l v t).(rlm) ≡ {[t]}.
+Proof.
+  intros t1.
+  rewrite elem_of_dom /res_mapsto lookup_op /= right_id elem_of_singleton
+          /to_lmUR lookup_fmap.
   case (decide (t1 = t)) => ?.
   - subst t1. rewrite lookup_insert. naive_solver.
   - rewrite lookup_insert_ne // lookup_empty. split; [by destruct 1|done].
